theories/ftlr/JmpCap.v
@@ -1,0 +1,109 @@
+From iris.proofmode Require Import proofmode.
+From iris.program_logic Require Import weakestpre adequacy lifting.
+From stdpp Require Import base.
+From cap_machine Require Export logrel.
+From cap_machine.ftlr Require Import ftlr_base.
+From cap_machine.rules Require Import rules_JmpCap.
+From cap_machine.proofmode Require Import map_simpl register_tactics.
+
+Section fundamental.
+  Context
+    {Σ:gFunctors}
+    {ceriseg:ceriseG Σ} {sealsg: sealStoreG Σ}
+    {Cname : CmptNameG}
+    {stsg : STSG Addr region_type Σ} {heapg : heapGS Σ}
+    {nainv: logrel_na_invs Σ}
+    `{MP: MachineParameters}.
+
+  Notation STS := (leibnizO (STS_states * STS_rels)).
+  Notation STS_STD := (leibnizO (STS_std_states Addr region_type)).
+  Notation CVIEW := (prodO STS_STD STS).
+  Notation WORLD := (gmapO CmptName CVIEW).
+  Implicit Types WC : CVIEW.
+  Implicit Types W : WORLD.
+  Implicit Types C : CmptName.
+
+  Notation D := (WORLD -n> (leibnizO CmptName) -n> (leibnizO Word) -n> iPropO Σ).
+  Notation R := (WORLD -n> (leibnizO CmptName) -n> (leibnizO Reg) -n> iPropO Σ).
+  Implicit Types w : (leibnizO Word).
+  Implicit Types interp : (D).
+
+
+  Lemma jmpcap_case (W : WORLD) (C : CmptName) (regs : leibnizO Reg)
+    (p p': Perm) (g : Locality) (b e a : Addr)
+    (w : Word) (ρ : region_type) (rsrc : RegName) (P:D):
+    ftlr_instr W C regs p p' g b e a w (JmpCap rsrc) ρ P.
+  Proof.
+    intros Hp Hsome HcorrectPC Hbae Hfp HO Hpers Hpwl Hregion Hnotrevoked Hnotfrozen Hi.
+    iIntros "#IH #Hinv_interp #Hreg #Hinva #Hrcond #Hwcond #Hmono #HmonoV Hw Hsts Hown".
+    iIntros "Hr Hstate Ha HPC Hmap".
+    destruct (decide (rsrc = PC)) as [HrPC|HrPC].
+    - subst rsrc.
+      iApply (wp_jmpcap_successPC with "[HPC Ha]"); eauto; first iFrame.
+      iNext. iIntros "[HPC Ha] /=".
+      iApply wp_pure_step_later; auto.
+      (* reconstruct regions *)
+      iNext; iIntros "_".
+      iInsert "Hmap" PC.
+      (* close region *)
+      iDestruct (region_close with "[$Hstate $Hr Hw $Ha $HmonoV]") as "Hr"; eauto.
+      { destruct ρ;auto;[|specialize (Hnotfrozen g0)];contradiction. }
+      (* apply IH *)
+      iApply ("IH" $! _ _ _ _ g _ _ a with "[] [] [Hmap] [$Hr] [$Hsts] [$Hown]"); eauto.
+      { iPureIntro; apply Hsome. }
+      destruct p
+      ; iFrame
+      ; apply isCorrectPC_nonSentry in HcorrectPC; by cbn in HcorrectPC.
+    - specialize Hsome with rsrc as Hrsrc; destruct Hrsrc as [wsrc Hsomesrc].
+      iExtract "Hmap" rsrc as "Hrsrc".
+      iApply (wp_jmpcap_success with "[$HPC $Ha $Hrsrc]"); eauto.
+      iNext. iIntros "[HPC [Ha Hrsrc]] /=".
+      iApply wp_pure_step_later; auto.
+      (* reconstruct regions *)
+      iInsert "Hmap" rsrc;
+      rewrite -delete_insert_ne; auto.
+      destruct (updatePcPerm wsrc) eqn:Heq ; [ | destruct sb | ]; cycle 1.
+      { destruct (executeAllowed p0) eqn:Hpft; cycle 1.
+        { iNext; iIntros "_".
+          iApply (wp_bind (fill [SeqCtx])).
+          iApply (wp_notCorrectPC with "HPC"); [eapply not_isCorrectPC_perm; naive_solver|].
+          iNext; iIntros "HPC /=".
+          iApply wp_pure_step_later; auto; iNext; iIntros "_".
+          iApply wp_value; iIntros; discriminate.
+        }
+        iInsert "Hmap" PC.
+        rewrite (insert_id regs rsrc); auto.
+        iDestruct ("Hreg" $! rsrc _ HrPC Hsomesrc) as "Hwsrc".
+        destruct wsrc; simpl in Heq; try congruence.
+        destruct sb as [p1 g1 b1 e1 a1|?]; try congruence.
+        destruct p1 as [rx pw dl dro | rx pw dl dro] ; cycle 1; simplify_eq.
+        + (* case p1 = E *)
+          iEval (rewrite fixpoint_interp1_eq) in "Hwsrc".
+          simpl; rewrite /enter_cond.
+          iDestruct "Hwsrc" as "#H".
+          iAssert (future_world g0 W W C) as "Hfuture".
+          { iApply futureworld_refl. }
+          iSpecialize ("H" with "Hfuture").
+          iDestruct "H" as "[H _]".
+          iDestruct (region_close with "[$Hstate $Hr Hw $Ha $HmonoV]") as "Hr"; eauto.
+          { destruct ρ;auto;[|ospecialize (Hnotfrozen _)];contradiction. }
+          iDestruct ("H" with "[$Hmap $Hr $Hsts $Hown]") as "HA"; eauto.
+          iFrame "#%".
+        + (* case p1 ≠ E *)
+          iEval (rewrite fixpoint_interp1_eq) in "Hinv_interp".
+          iNext; iIntros "_".
+          iDestruct (region_close with "[$Hstate $Hr Hw $Ha $HmonoV]") as "Hr"; eauto.
+          { destruct ρ;auto;[|ospecialize (Hnotfrozen _)];contradiction. }
+          iApply ("IH" with "[] [] [$Hmap] [$Hr] [$Hsts] [$Hown]"); eauto.
+      }
+
+      (* Non-capability cases *)
+      all: iNext; iIntros "_".
+      all: iApply (wp_bind (fill [SeqCtx])).
+      all: iApply (wp_notCorrectPC with "HPC"); [intro Hcontra ; inv Hcontra|].
+      all: iNext; iIntros "HPC /=".
+      all: iApply wp_pure_step_later; auto; iNext; iIntros "_".
+      all: iApply wp_value; iIntros; discriminate.
+  Qed.
+
+End fundamental.
